Machines.lean
@@ -1,5 +1,5 @@
 import Machines.Acc8.Theorems.A1
 import Machines.Acc8.Iss
 import Machines.Acc8.DslRegression
-import Machines.Lnp64u.Theorems.T1
+import Machines.Lnp64u.Theorems.Ledger
 import Machines.Lnp64u.Iss
